add more exercise

Chapter8.v
@@ -209,4 +209,218 @@ Lemma le_my_le : forall n p:nat, le n p -> my_le n p.
   induction H;
   auto.
 Qed.
+Require Export Program.
+Inductive par := open | close.
+Inductive wp : list par -> Prop :=
+| wp_nil : wp []
+| wp_par l : wp l -> wp (open :: (l ++ [close]))
+| wp_app l r : wp l -> wp r -> wp (l ++ r).
+Hint Constructors wp.
 
+Theorem cons_app { A } (l : A) r : l :: r = [l] ++ r.
+  trivial.
+Qed.
+
+Theorem wp_oc : wp [open;close].
+  rewrite (cons_app open); repeat constructor.
+Qed.
+
+Theorem wp_o_head_c l1 l2 : wp l1 -> wp l2 -> wp (open :: l1 ++ close :: l2).
+  intros; rewrite (cons_app open), (cons_app close).
+  rewrite !app_assoc; apply wp_app; simpl; auto.
+Qed.
+
+Theorem wp_o_tail_c l1 l2 : wp l1 -> wp l2 -> wp (l1 ++ open :: l2 ++ [close]).
+  intros; rewrite (cons_app open).
+  apply wp_app; simpl; auto.
+Qed.
+
+Fixpoint recognize n (l : list par) : bool :=
+  match l, n with
+  | [], 0 => true
+  | open :: l', _ => recognize (S n) l'
+  | close :: l', S n' => recognize n' l'
+  | _, _ => false
+  end.
+
+Theorem repeat_shift { A } (e : A) n : repeat e n ++ [e] = e :: repeat e n.
+  induction n; simpl in *; f_equal; auto.
+Qed.
+
+Theorem get_last { A } (l : list A) : l = [] \/ exists l' e, l = l' ++ [e].
+  induction l; intuition idtac; program_simpl.
+  right; exists (@nil A) a; trivial.
+  right; exists (a :: H) H0; trivial.
+Qed.
+Hint Resolve wp_oc.
+
+Inductive wp' : list par -> Prop :=
+| wp'_nil : wp' []
+| wp'_cons l r : wp' l -> wp' r -> wp' (open :: l ++ close :: r).
+Hint Constructors wp'.
+Theorem wp'_app l r : wp' l -> wp' r -> wp' (l ++ r).
+  intros HL HR; induction HL; simpl in *; auto.
+  rewrite <- app_assoc, <- app_comm_cons; auto.
+Qed.
+Hint Resolve wp'_app.
+Theorem wp_wp' l : wp l -> wp' l.
+  induction 1; simpl in *; auto.
+Qed.
+
+Theorem wp'_wp l : wp' l -> wp l.
+  induction 1; auto.
+  replace (open :: l ++ close :: r) with ((open :: l ++ [close]) ++ r); auto.
+  simpl; f_equal; rewrite <- app_assoc; trivial.
+Qed.
+
+Hint Resolve wp_wp' wp'_wp.
+
+Require Export Omega.
+
+Theorem wp_close_false l : wp (close :: l) -> False.
+  intros H; dependent induction H.
+  destruct l0; inversion x; simpl in *; subst; eauto.
+Qed.
+
+Theorem wp_open_false l : wp (l ++ [open]) -> False.
+  intros H; dependent induction H; destruct l; program_simpl.
+  destruct l0; program_simpl.
+  apply app_inj_tail in H2; intuition congruence.
+  destruct l0, r; program_simpl.
+  specialize(IHwp2 []); program_simpl.
+  destruct l0; specialize(IHwp1 []); program_simpl.
+  destruct l0, p0; program_simpl.
+  destruct (get_last r); program_simpl; rewrite ?app_nil_r in *; subst; eauto.
+  rewrite app_assoc in *; apply app_inj_tail in x; intuition; program_simpl; eauto.
+Qed.
+
+Hint Resolve wp_close_false wp_open_false.
+
+Theorem wp_app_inv n l : length l < n -> wp (open :: close :: l) -> wp l.
+  revert l; induction n; intros; [omega|].
+  apply wp_wp' in H0; inversion H0; clear H0; simpl in *.
+  destruct l0; simpl in *; program_simpl.
+  apply wp'_wp in H2; exfalso; eauto.
+Qed.
+
+Ltac invcs s := inversion s; clear s; subst.
+Theorem par_destruct_aux n l : length l < n -> head l = Some open -> 
+  (exists n, l = repeat open n) \/ (exists n li, l = repeat open n ++ close :: li).
+  revert l; induction n; intros; simpl in *; [omega|].
+  destruct l as [|[]]; simpl in *; invcs H0.
+  destruct l as [|[]]; simpl in *.
+  left; exists 1; trivial.
+  destruct (IHn (open :: l)) as [[]|[? []]]; simpl in *; omega || trivial;
+  destruct x; simpl in *; invcs H0.
+  left; exists (S (S x)); trivial.
+  right; exists (S (S x)) x0; trivial.
+  right; exists 1 l; trivial.
+Qed.
+
+Theorem par_destruct l :
+  (exists n, l = repeat open n) \/ (exists n li, l = repeat open n ++ close :: li).
+  destruct l as [|[]].
+  left; exists 0; trivial.
+  destruct (par_destruct_aux (S (S (length l))) (open :: l)); 
+  simpl in *; program_simpl; omega || trivial.
+  destruct H; invcs H0.
+  left; exists (S H); trivial.
+  destruct H; simpl in *; invcs H1.
+  right; exists (S H) H0; trivial.
+  right; exists 0 l; trivial.
+Qed.
+
+Theorem length_eq { A } { l r : list A } (H : l = r) : length l = length r.
+  subst; trivial.
+Qed.
+
+Theorem app_eq { A } { ll lr rl rr : list A } : 
+  ll ++ lr = rl ++ rr -> exists l, ll = rl ++ l \/ rl = ll ++ l.
+  revert lr rl rr.
+  induction ll; program_simpl; eauto.
+  destruct rl; simpl in *; invcs H; eauto.
+  specialize(IHll _ _ _ H2); program_simpl; intuition idtac; subst; eauto.
+Qed.
+
+Theorem wp_remove_aux n : forall l r, length l + length r < n ->
+  wp (l ++ [open; close] ++ r) -> wp (l ++ r).
+  induction n; simpl in *; intros; [omega|].
+  apply wp_wp' in H0; invcs H0.
+  destruct l; simpl in *; congruence.
+  destruct l; simpl in *; invcs H1.
+  destruct l0; simpl in *; invcs H4; eauto with *.
+  destruct (app_eq H5) as [? []]; subst;
+  rewrite <- app_assoc in *;
+  apply app_inv_head in H5.
+  destruct x; invcs H5.
+  destruct x; invcs H4; try solve [exfalso; eauto].
+  apply wp'_wp in H2; eapply IHn in H2; 
+  repeat (simpl in *; rewrite ?app_length in *); try omega.
+  replace 
+    (open :: l ++ x ++ close :: r0) with 
+    ((open :: l ++ x ++ [close]) ++ r0) by
+    (simpl; f_equal; rewrite <- app_assoc; f_equal; rewrite <- app_assoc; trivial).
+  apply wp_app; auto.
+  rewrite app_assoc; auto.
+  destruct x; simpl in *; invcs H5.
+  replace 
+    (open :: l0 ++ close :: x ++ r) with 
+    ((open :: l0 ++ [close]) ++ x ++ r) by
+    (simpl; f_equal; rewrite <- app_assoc; f_equal).
+  apply wp_app; auto.
+  eapply IHn; repeat (simpl in *; rewrite ?app_length in *); omega || auto.
+Qed.
+
+Theorem wp_remove l r : wp (l ++ open :: close :: r) -> wp (l ++ r).
+  intros; eapply wp_remove_aux; auto.
+Qed.
+
+Theorem recognize_complete_aux l : wp l -> forall n l', recognize n (l ++ l') = recognize n l'.
+  induction 1; intros; simpl in *; rewrite <- ?app_assoc, ?IHwp, ?IHwp1, ?IHwp2; trivial.
+Qed.
+
+Theorem recognize_complete l : wp l -> recognize 0 l = true.
+  induction 1; simpl in *; rewrite ?recognize_complete_aux; trivial.
+Qed.
+
+Theorem wp_destruct l : wp l -> 
+  l = [] \/ 
+  (exists l1 l2, l = l1 ++ l2 /\ wp l1 /\ wp l2 /\ l1 <> [] /\ l2 <> []) \/ 
+  (exists l1, l = open :: l1 ++ [close] /\ wp l1).
+  induction 1; intros; try solve [intuition idtac].
+  right; right; exists l; intuition.
+  destruct IHwp1; program_simpl; simpl in *; trivial.
+  destruct IHwp2; program_simpl; simpl in *; rewrite ?app_nil_r in *; eauto.
+  right; left; exists l r; intuition idtac; program_simpl;
+  match goal with H : ?X ++ ?Y = [] |- _ => destruct X; simpl in *; congruence end.
+Qed.
+
+Theorem wp_insert : forall n a b c, 
+  length a + length b + length c < n -> wp (a ++ c) -> wp b -> wp (a ++ b ++ c).
+  induction n; intros; simpl in *; [omega|].
+  apply wp_destruct in H0; intuition idtac; program_simpl.
+  + destruct a, c; simpl in *; rewrite ?app_nil_r; congruence.
+  + destruct (app_eq H3); intuition idtac; subst; rewrite <- app_assoc in *;
+    apply app_inv_head in H3; subst; repeat (simpl in *; rewrite ?app_length in *).
+    - apply wp_app; eauto.
+      eapply IHn; eauto.
+      destruct H0; simpl in *; congruence || omega.
+    - rewrite !app_assoc; apply wp_app; eauto.
+      rewrite <- app_assoc; eapply IHn; eauto.
+      destruct H2; simpl in *; congruence || omega.
+  + destruct a; simpl in *; invcs H2; eauto.
+    destruct (get_last c); program_simpl;
+    repeat (rewrite ?app_nil_r, ?app_length, <- ?plus_n_O in *; subst; simpl in *).
+    - rewrite app_comm_cons; eauto.
+    - rewrite app_assoc in H6; apply app_inj_tail in H6; intuition idtac; subst.
+      rewrite !app_assoc; apply wp_par; rewrite <- app_assoc; eapply IHn; eauto; omega.
+Qed.
+
+Theorem recognize_sound n l : recognize n l = true -> wp ((repeat open n) ++ l).
+  revert n; induction l; intros; simpl in *.
+  destruct n; simpl; congruence || auto.
+  destruct a, n; simpl in *; try specialize (IHl _ H); simpl in *; congruence || auto.
+  rewrite (cons_app _ l), app_assoc, repeat_shift; simpl; trivial.
+  rewrite app_comm_cons, <- repeat_shift, <- app_assoc, (cons_app _ l), (app_assoc _ _ l).
+  eapply wp_insert; eauto.
+Qed.
